Tests/examples/DQueue.tla
@@ -1,0 +1,47 @@
+\* https://github.com/DistCompiler/pgo/blob/main/systems/dqueue/dqueue.tla
+
+------------ MODULE DQueue ---------------
+EXTENDS Fugue
+
+CONSTANTS
+  \* @type: () => Str;
+  Stream,
+  \* @type: Set(Address);
+  Nodes,
+  \* @type: Address;
+  Producer
+
+(*--algorithm DQueue {
+  fifos
+    \* @type: Channel(Address);
+    producer,
+    \* @type: Address -> Channel(Str);
+    consumer[Nodes];
+
+  \* @mailbox: producer;
+  process (Producer = Producer)
+    variable
+      \* @type: Address;
+      addr = self;
+  {
+  p:  while (TRUE) {
+  p1:   receive(producer, addr);
+  p2:   send(consumer[addr], Stream());
+      }
+  }
+
+  \* @mailbox: consumer[self];
+  process (Consumer \in Nodes)
+    variable
+      \* @type: Str;
+      msg;
+  {
+  c:  while (TRUE) {
+  c1:   send(producer, self);
+  c2:   receive(consumer[self], msg);
+        print msg;
+      }
+  }
+}*)
+
+==========
